theories/contexts.v
@@ -2,16 +2,15 @@
     additional context stack to replace the inductive definition, since the evaluation context tree is
     guaranteed to be linear. **)
 
-From mathcomp Require Import ssreflect ssrfun ssrnat ssrbool eqtype seq.
+From mathcomp Require Import ssreflect ssrnat ssrbool eqtype seq.
 From HB Require Import structures.
 From Coq Require Import Program NArith ZArith Wf_nat.
-From Wasm Require Export common operations datatypes_properties properties opsem typing_inversion tactic.
+From Wasm Require Export common operations datatypes_properties properties opsem typing_inversion tactic wasm_parray.
 Require Import FunInd Recdef.
 
 Set Implicit Arguments.
 Unset Strict Implicit.
 Unset Printing Implicit Defensive.
-
 
 Section EvalContext.
 
